More progress

theories/Lowering/ParallelMove.v
@@ -46,6 +46,46 @@ Proof.
   cset_tac.
 Qed.
 
+Instance eqdec_pospos
+  :EqDec (positive * positive) eq.
+hnf; intros.
+decide (x === y). left. invc e. rewrite H, H0. reflexivity.
+right; intro. invc H. eauto.
+Defined.
+
+Instance eqdec_pos
+  :EqDec (positive) eq.
+hnf; intros.
+decide (x === y); eauto.
+Defined.
+
+Lemma fst_parmove x pm
+  : of_list (fst ⊝ Parmov.parmove positive var_dec (fun _ : positive => x) pm) ⊆ {x; of_list (fst ⊝ pm)}.
+Proof.
+  hnf; intros.
+  eapply of_list_get_first in H; dcr. invc H1.
+  eapply get_in in H0; eauto.
+  eapply Parmov.parmove_srcs_initial_reg_or_temp in H0.
+  destruct H0. eapply in_get in H; dcr.
+  unfold Parmov.srcs in p. eapply get_in_of_list in p. cset_tac.
+  eapply eqdec_pos.
+  destruct H; subst. cset_tac.
+  eapply eqdec_pos.
+Qed.
+
+Lemma snd_parmove x pm
+  : of_list (snd ⊝ Parmov.parmove positive var_dec (fun _ : positive => x) pm) ⊆ {x; of_list (snd ⊝ pm)}.
+Proof.
+  hnf; intros.
+  eapply of_list_get_first in H; dcr. invc H1.
+  eapply get_in in H0; eauto.
+  eapply Parmov.parmove_dests_initial_reg_or_temp in H0.
+  destruct H0. eapply in_get in H; dcr.
+  unfold Parmov.dests in p. eapply get_in_of_list in p. cset_tac.
+  eapply eqdec_pos.
+  destruct H; subst. cset_tac.
+  eapply eqdec_pos.
+Qed.
 
 Lemma combine_get A B (Z:list A) (Y:list B) n x y
   : get Z n x -> get Y n y -> get (combine Z Y) n (x,y).
@@ -59,34 +99,31 @@ Lemma move_no_temp_notin m pmtmp
   : pmtmp ∉ of_list (fst ⊝ m) ∪ of_list (snd ⊝ m)
     <-> Parmov.move_no_temp positive (fun _ : positive => pmtmp) m.
 Proof.
-  assert (EqDec:EqDec (positive * positive) eq). {
-    hnf; intros.
-    decide (x === y). left. invc e. rewrite H, H0. reflexivity.
-    right; intro. invc H. eauto.
-  }
   split; hnf; intros; hnf; intros.
   - split; hnf; intros.
     + eapply in_get in H0 as [? ?]; eauto.
       hnf; intros; subst.
       cset_tac'. eapply H0.
       eapply get_in_of_list.
-      eapply map_get_eq; eauto.
+      eapply map_get_eq; eauto. eauto with typeclass_instances.
     + eapply in_get in H0 as [? ?]; eauto.
       hnf; intros; subst.
       cset_tac'. eapply H1.
       eapply get_in_of_list.
-      eapply map_get_eq; eauto.
+      eapply map_get_eq; eauto. eauto with typeclass_instances.
   - cset_tac'.
     + edestruct of_list_get_first; eauto; dcr. invc H2.
       inv_get.
       exploit (H (fst x1) (snd x1)).
       eapply get_in; eauto using combine_get; eauto.
+      * eauto with typeclass_instances.
       * rewrite <- pair_eta; eauto.
       * dcr. eapply H2; eauto. eapply 1%positive.
     + edestruct of_list_get_first; eauto; dcr. invc H2.
       inv_get.
       exploit (H (fst x1) (snd x1)).
       eapply get_in; eauto using combine_get; eauto.
+      * eauto with typeclass_instances.
       * rewrite <- pair_eta; eauto.
       * dcr. eapply H4; eauto. eapply 1%positive.
 Qed.
@@ -127,15 +164,6 @@ Section ParmovSourceSet.
     - etransitivity; eauto.
   Qed.
 
-  Lemma dtransitions_dst_set t st st'
-    : dtransitions var t st st' ->
-      st_source_set st' ⊆ st_source_set st.
-  Proof.
-    intros TR.
-    general induction TR; simpl in *; eauto using dtransition_source_set.
-    - etransitivity; eauto.
-  Qed.
-
   Lemma parmove_src_set t mu
     : moves_source_set (parmove var var_dec t mu) ⊆ of_list (fst ⊝ mu).
   Proof.
@@ -146,6 +174,58 @@ Section ParmovSourceSet.
   Qed.
 
 End ParmovSourceSet.
+
+Section ParmovDestinationSet.
+  Import Parmov.
+
+  Definition st_dest_set x (st:state var) :=
+    match st with
+    | State mv1 mv2 mvs => of_list (snd ⊝ (mv1 ++ mv2 ++ mvs))
+                                  \ (of_list (fst ⊝ (mv1 ++ mv2 ++ mvs))
+                                             ∪ singleton x)
+    end.
+
+  Tactic Notation "stsmpl" :=
+    repeat (rewrite List.map_app || rewrite of_list_app || simpl).
+
+  Lemma dtransition_dest_set x st st'
+    : dtransition var (fun _ => x) st st' ->
+      st_dest_set x st ⊆ st_dest_set x st'.
+  Proof.
+    intros TR.
+    general induction TR; simpl in *; eauto; stsmpl.
+    - cset_tac.
+    - cset_tac.
+    - cset_tac.
+    - cset_tac.
+    - cset_tac.
+   Qed.
+
+  Lemma dtransitions_dest_set x st st'
+    : dtransitions var (fun _ => x) st st' ->
+      st_dest_set x st ⊆ st_dest_set x st'.
+  Proof.
+    intros TR.
+    general induction TR; simpl in *; eauto.
+    - eapply dtransition_dest_set; eauto.
+    - etransitivity; eauto.
+  Qed.
+
+  Lemma parmove_dest_set (x:var) mu
+        (NOTIN:x ∉ of_list (snd ⊝ mu))
+    : of_list (snd ⊝ mu) \ of_list (fst ⊝ mu) ⊆ moves_dest_set (parmove var var_dec (fun _ => x) mu).
+  Proof.
+    pose proof (parmove_aux_transitions _ var_dec (fun _ => x) (State _ mu nil nil)).
+    eapply dtransitions_dest_set in H.
+    simpl in *. revert H; stsmpl.
+    unfold parmove, moves_dest_set.
+    rewrite map_rev. rewrite of_list_rev.
+    intros.
+    cset_tac.
+  Qed.
+
+End ParmovDestinationSet.
+
 
 Lemma eq_dec_comm X (x y:X)
   : { x = y } + { ~ x = y }
@@ -275,6 +355,36 @@ Proof.
   - right; eauto.
 Qed.
 
+Fixpoint parmove_elim_mem2mem (p:inf_partition var) (r:var) (pm:〔var * var〕) :=
+  match pm with
+  | (x,y)::pm => if [part_2 p x /\ part_2 p y] then (x,r)::(r,y)::parmove_elim_mem2mem p r pm
+                else (x,y)::parmove_elim_mem2mem p r pm
+  | nil => nil
+  end.
+
+Lemma moves_source_set_elim_mem2mem p (r:var) pm
+      (NOTIN: r ∉ of_list (fst ⊝ pm) ∪ of_list (snd ⊝ pm))
+  : moves_source_set (parmove_elim_mem2mem p r pm) [=] moves_source_set pm.
+Proof.
+  general induction pm; simpl; eauto.
+  pose proof (moves_source_set_incl pm) as INCL.
+  destruct a; simpl; cases; simpl in *; rewrite IHpm.
+  - clear - NOTIN INCL; cset_tac.
+  - clear - NOTIN; cset_tac.
+  - clear - NOTIN INCL; cset_tac.
+  - clear - NOTIN; cset_tac.
+Qed.
+
+Lemma moves_dest_set_elim_mem2mem p (r:var) pm
+  : moves_dest_set pm ⊆ moves_dest_set (parmove_elim_mem2mem p r pm).
+Proof.
+  unfold moves_dest_set.
+  general induction pm; simpl; eauto.
+  destruct a; simpl; cases; simpl in *; rewrite IHpm.
+  - clear; cset_tac.
+  - clear; cset_tac.
+Qed.
+
 Fixpoint lower (p:inf_partition var) (preg:var) (DL:〔⦃var⦄ * params〕) s (an:ann (set var))
   : stmt :=
   match s, an with
@@ -284,14 +394,22 @@ Fixpoint lower (p:inf_partition var) (preg:var) (DL:〔⦃var⦄ * params〕) s 
       let '(lv', Z) := nth_default (∅, nil) DL (counted l) in
       let x := least_fresh_P (part_2 p) (lv' ∪ lv) in
       let z := least_fresh_P (part_2 p) ({x; lv'} ∪ lv) in
-      let r := least_fresh_P (part_1 p) (lv' \ of_list Z ∪ lv) in
+      let r := least_fresh_P (part_1 p) (lv' ∪ lv) in
       if [ (r <= preg)%positive ] then
         let mvs := Parmov.parmove2 var var_dec (fun _ => x) (onlyVars Y) Z in
-        list_to_stmt mvs (stmtApp l nil)
+        let mvs' := parmove_elim_mem2mem p r mvs in
+        list_to_stmt mvs' (stmtApp l nil)
       else
-        let r := proj1_sig (InfiniteSubset.inf_subset_least (part_1 p)) in
-        let mvs := Parmov.parmove2 var var_dec (fun _ => x) (repl (onlyVars Y) r z) (repl Z r z) in
-        list_to_stmt ((r,z)::mvs++(z,r)::nil) (stmtApp l nil)
+        let r := least_fresh_P (part_1 p) lv in
+        if [ (r <= preg)%positive ] then
+          let mvs := Parmov.parmove2 var var_dec (fun _ => x) (onlyVars Y) (repl Z r z) in
+          let mvs' := parmove_elim_mem2mem p r mvs in
+          list_to_stmt (mvs'++(z,r)::nil) (stmtApp l nil)
+        else
+          let r := proj1_sig (InfiniteSubset.inf_subset_least (part_1 p)) in
+          let mvs := Parmov.parmove2 var var_dec (fun _ => x) (repl (onlyVars Y) r z) (repl Z r z) in
+          let mvs' := parmove_elim_mem2mem p r mvs in
+          list_to_stmt ((r,z)::mvs'++(z,r)::nil) (stmtApp l nil)
     | stmtReturn x, ann0 lv => stmtReturn x
     | stmtFun F t, annF lv ans ant =>
       let DL' := pair ⊜ (getAnn ⊝ ans) (fst ⊝ F) in
@@ -377,6 +495,34 @@ Proof.
   - rewrite IHZ; cset_tac.
 Qed.
 
+Lemma of_list_repl Z x y
+  : of_list (repl Z x y) ⊆ {y; of_list Z \ singleton x}.
+Proof.
+  general induction Z; simpl; repeat cases; eauto.
+  - cset_tac.
+  - rewrite IHZ; cset_tac.
+  - rewrite IHZ; cset_tac.
+Qed.
+
+Lemma of_list_repl_eq (Z:params) x y
+      (IN: x ∈ of_list Z)
+  : of_list (repl Z x y) [=] {y; of_list Z \ singleton x}.
+Proof.
+  general induction Z; simpl; repeat cases; simpl in *; eauto.
+  - invc COND. decide (a ∈ of_list Z).
+    + rewrite IHZ; cset_tac.
+    + rewrite repl_not_in; eauto. cset_tac.
+  - rewrite IHZ; cset_tac.
+Qed.
+
+Lemma of_list_repl' Z x y
+  : of_list Z \ singleton x ⊆ of_list (repl Z x y).
+Proof.
+  general induction Z; simpl; repeat cases; eauto.
+  - rewrite <- IHZ; cset_tac.
+  - rewrite <- IHZ; cset_tac.
+Qed.
+
 Lemma repl_get_ne (Z:params) n (x y z:var)
   : get Z n z -> z =/= x -> get (repl Z x y) n z.
 Proof.
@@ -396,14 +542,52 @@ Proof.
   general induction Z; simpl in *; repeat cases in GET; inv GET; eauto using get.
 Qed.
 
-Lemma parmov_repl_agree lv (E:onv val) (pmtmp reg lstmp:var) (Y Z:params) (Len:❬Y❭=❬Z❭) (NEQ:reg =/= lstmp) (NEQ2:pmtmp =/= lstmp)
+Lemma exec_seq_agree G pm (E E':onv val)
+      (AGR: agree_on eq (G ∪ moves_source_set pm) E E')
+  : agree_on eq G (E <||= pm) (E' <||= pm).
+Proof.
+  general induction pm; simpl in *; eauto.
+  - eapply agree_on_incl; eauto.
+  - destruct a. rewrite !Parmov_update_eq.
+    eapply IHpm. simpl in *.
+    eapply agree_on_update_same.
+    eapply AGR; eauto.
+    cset_tac.
+    eapply agree_on_incl; eauto.
+    cset_tac.
+Qed.
+
+
+Lemma parmove_elim_mem2mem_agree G (p:inf_partition var) (reg:var) (E':onv val) pm
+      (NOTIN:reg ∉ of_list (fst ⊝ pm))
+  : agree_on eq (G \ singleton reg)
+             (E' <||= parmove_elim_mem2mem p reg pm)
+             (E' <||= pm).
+Proof.
+  general induction pm; simpl.
+  - reflexivity.
+  - destruct a; cases; simpl; rewrite !Parmov_update_eq.
+    + etransitivity.
+      eapply IHpm. simpl in *. cset_tac.
+      lud; eauto.
+      eapply exec_seq_agree.
+      hnf; intros. lud.
+      invc H3. exfalso.
+      rewrite moves_source_set_incl in H. simpl in *.
+      cset_tac.
+    + eapply IHpm. simpl in *. cset_tac.
+Qed.
+
+Lemma parmov_repl_agree p lv (E:onv val) (pmtmp reg lstmp:var) (Y Z:params) (Len:❬Y❭=❬Z❭) (NEQ:reg =/= lstmp) (NEQ2:pmtmp =/= lstmp) (NEQ3:reg =/= pmtmp)
       (NDZ:NoDupA _eq Z) (NOTIN:lstmp ∉ of_list Y ∪ of_list Z) (NOTIN2: pmtmp ∉ of_list Y ∪ of_list Z)
   : agree_on eq (lv \ {lstmp; singleton pmtmp})
              (E <||= Parmov.parmove2 positive var_dec (fun _ : positive => pmtmp) Y Z)
              (E <||=
                 ((reg, lstmp)
-                   :: Parmov.parmove2 positive var_dec (fun _ : positive => pmtmp) (repl Y reg lstmp)
-                   (repl Z reg lstmp) ++ (lstmp, reg) :: nil)).
+                   ::
+                   parmove_elim_mem2mem p reg
+                   (Parmov.parmove2 positive var_dec (fun _ : positive => pmtmp) (repl Y reg lstmp)
+                                    (repl Z reg lstmp)) ++ (lstmp, reg) :: nil)).
 Proof.
   simpl; rewrite Parmov.exec_seq_app; simpl.
   rewrite !Parmov_update_eq.
@@ -420,6 +604,13 @@ Proof.
   }
   symmetry. etransitivity. {
     eapply agree_on_update_same. reflexivity.
+    eapply parmove_elim_mem2mem_agree.
+    unfold Parmov.parmove2.
+    rewrite fst_parmove. rewrite fst_combine; eauto with len.
+    subst YR. rewrite of_list_repl. cset_tac.
+  }
+  etransitivity. {
+    eapply agree_on_update_same. reflexivity.
     eapply agree_on_incl.
     eapply parmov_update_with_list; eauto.
     + rewrite snd_combine; eauto with len.
@@ -430,33 +621,37 @@ Proof.
   }
   symmetry.
   rewrite snd_combine, fst_combine; eauto with len.
+  erewrite parmove_elim_mem2mem_agree with (G:=singleton lstmp);
+    [|unfold Parmov.parmove2; rewrite fst_parmove; try rewrite fst_combine; eauto with len;
+      subst YR; rewrite of_list_repl; cset_tac
+     |cset_tac].
   hnf; intros. lud.
   - unfold Parmov.parmove2.
     erewrite parmov_update_with_list; eauto;
       try rewrite snd_combine; try rewrite fst_combine; eauto with len.
-    + invc H2; clear e.
+    + invc H3; clear e.
       decide (reg ∈ of_list Z).
-      * eapply of_list_get_first in i; dcr. symmetry in H5; invc H5.
+      * eapply of_list_get_first in i; dcr. symmetry in H8; invc H8.
         exploit (@update_with_list_lookup_in_list_first _ _ _ E x Z (lookup_list E Y)); dcr;
           eauto with len.
-        rewrite H9. rewrite lookup_list_map in H8. inv_get. rewrite <- EQ.
-        exploit repl_get_eq; try eapply H2; eauto.
+        rewrite H12. rewrite lookup_list_map in H11. inv_get. rewrite <- EQ.
+        exploit repl_get_eq; try eapply H3; eauto.
         exploit (@update_with_list_lookup_in_list_first _ _ _ (E [lstmp <- E reg]) x ZR (lookup_list (E [lstmp <- E reg]) YR)); dcr;
           eauto with len.
-        -- intros. intro. invc H6.
-           unfold ZR in H5. unfold repl in H5. inv_get. cases in EQ0.
-           ++ eapply H7. eauto. eauto. eauto.
+        -- intros. intro. invc H7.
+           unfold ZR in H6. unfold repl in H6. inv_get. cases in EQ0.
+           ++ eapply H10. eauto. eauto. eauto.
            ++ subst.
-             eapply get_in_of_list in H5. cset_tac.
-        -- rewrite H9.
-           rewrite lookup_list_map in H6. subst YR. unfold repl in H6.
-           inv_get. cases in H4.
+             eapply get_in_of_list in H6. cset_tac.
+        -- rewrite H8.
+           rewrite lookup_list_map in H7. subst YR. unfold repl in H7.
+           inv_get. cases in H5.
            ++ invc COND.
-             rewrite <- H4. lud. cset_tac.
-           ++ unfold repl in H3. inv_get.
-             cases in H3.
-             rewrite <- H4. lud. invc H6.
-             eapply get_in_of_list in H8. exfalso. cset_tac.
+             rewrite <- H5. lud. cset_tac.
+           ++ unfold repl in H4. inv_get.
+             cases in H4.
+             rewrite <- H5. lud. invc H7.
+             eapply get_in_of_list in H11. exfalso. cset_tac.
       * rewrite !lookup_set_update_not_in_Z; eauto.
         lud. cset_tac.
         subst ZR. rewrite repl_not_in; eauto. cset_tac.
@@ -465,28 +660,28 @@ Proof.
     + instantiate (1:=singleton lstmp). cset_tac.
   - rewrite fst_combine, snd_combine; eauto with len.
     decide (x ∈ of_list Z).
-    + eapply of_list_get_first in i; dcr. symmetry in H5; invc H5.
+    + eapply of_list_get_first in i; dcr. symmetry in H6; invc H6.
       exploit (@update_with_list_lookup_in_list_first _ _ _ E x0 Z (lookup_list E Y)); dcr;
         eauto with len.
-      rewrite H9.
-      rewrite lookup_list_map in H8. inv_get. rewrite <- EQ.
+      rewrite H10.
+      rewrite lookup_list_map in H9. inv_get. rewrite <- EQ.
       exploit repl_get_ne; try eapply H4; eauto.
       exploit (@update_with_list_lookup_in_list_first _ _ _ (E [lstmp <- E reg]) x0 ZR (lookup_list (E [lstmp <- E reg]) YR)); dcr;
         eauto with len.
       * subst ZR. intros. unfold repl in *. inv_get.
         repeat cases; eauto. invc COND.
-        intro. invc H5.
+        intro. invc H6.
         cset_tac.
-      * subst YR. rewrite lookup_list_map in H10.
-        unfold repl in H5, H10. inv_get.
+      * subst YR. rewrite lookup_list_map in H11.
+        unfold repl in H6, H11. inv_get.
         repeat cases; eauto.
-        cases in H6.
+        cases in H7.
         -- invc COND.
-           rewrite <- H6. lud; eauto.
-        -- rewrite <- H6. lud; eauto. invc H10. clear e.
-           exfalso. clear - H8 NOTIN.
-           eapply get_in_of_list in H8.
-           cset_tac'.
+           rewrite <- H7. lud; eauto.
+        -- rewrite <- H7. lud; eauto. invc H11. clear e.
+           exfalso. clear - H9 NOTIN.
+           eapply get_in_of_list in H9.
+           cset_tac.
     + rewrite !lookup_set_update_not_in_Z; eauto.
       lud. cset_tac.
       eapply repl_not_in'; eauto. cset_tac.
@@ -522,14 +717,15 @@ Proof.
     eapply op_eval_var in H5 as [Y' ?]; subst Y.
     rewrite onlyVars_idem in *. len_simpl.
     case_eq (omap (op_eval E) (Var ⊝ Y')); intros.
-    + set (reg:=least_fresh_P (part_1 p) (blv \ of_list Z0 ∪ lv)) in *.
+    + set (reg:=least_fresh_P (part_1 p) (blv ∪ lv)) in *.
+      set (reg2:=least_fresh_P (part_1 p) lv) in *.
       set (lreg:=InfiniteSubset.inf_subset_least (part_1 p)) in *.
       set (pmtmp := least_fresh_P (part_2 p) (blv ∪ lv)) in *.
       set (lstmp := least_fresh_P (part_2 p) ({pmtmp; blv} ∪ lv)) in *.
       assert (NEQ1:reg =/= lstmp). {
         subst reg lstmp.
         intro.
-        eapply (part_disj p (least_fresh_P (part_1 p) (blv \ of_list Z0 ∪ lv))); eauto.
+        eapply (part_disj p (least_fresh_P (part_1 p) (blv ∪ lv))); eauto.
         eapply least_fresh_P_full_spec.
         rewrite H5.
         eapply least_fresh_P_full_spec.
@@ -542,6 +738,12 @@ Proof.
       assert (NEQ3:proj1_sig lreg =/= lstmp). {
         subst lreg lstmp. destr_sig; dcr.
         intro. invc H7.
+        eapply (part_disj p); eauto.
+        eapply least_fresh_P_full_spec.
+      }
+      assert (NEQ4:proj1_sig lreg =/= pmtmp). {
+        subst lreg pmtmp. destr_sig; dcr.
+        intro. invc H5. simpl in *. dcr.
         eapply (part_disj p); eauto.
         eapply least_fresh_P_full_spec.
       }
@@ -560,17 +762,25 @@ Proof.
         setoid_rewrite union_comm at 2.
         setoid_rewrite <- incl_add' at 2. eauto.
       }
+      assert (reg ∉ getAnn al). {
+        intro.
+        eapply (least_fresh_P_full_spec (part_1 p) (blv ∪ lv)).
+        change (reg ∈ blv ∪ lv). clear - H7 INCL AL. cset_tac.
+      }
       unfold Parmov.srcs, Parmov.dests in *.
       exploit omap_op_eval_live_agree; try eassumption.
       {
-        cases.
+        repeat cases.
         - exploit (@list_to_stmt_correct
-                     (Parmov.parmove2 positive var_dec (fun _ : positive => pmtmp) Y' Z0)
+                     (parmove_elim_mem2mem p reg
+                                           (Parmov.parmove2 _ var_dec (fun _ => pmtmp) Y' Z0))
                      (stmtApp l nil) E' L'). {
             unfold Parmov.parmove2.
             simpl.
+            rewrite moves_source_set_elim_mem2mem.
             rewrite !parmove_src_set. rewrite fst_combine; eauto with len.
             eapply omap_var_defined_on; eauto.
+            admit.
           }
           pfold. eapply SimSilent.
           * eapply plus2O. econstructor; eauto with len. reflexivity.
@@ -580,73 +790,9 @@ Proof.
             -- eapply (inRel_drop LA H4).
             -- assert (getAnn al ⊆ blv) by eauto with cset.
                eapply agree_on_incl.
-               symmetry. etransitivity.
-               eapply (@parmov_update_with_list (getAnn al));
-                 try rewrite eauto.
-               ++ rewrite snd_combine; eauto.
-               ++ assert (of_list Y' ⊆ lv). {
-                   eapply Ops.freeVars_live_list in H3.
-                   rewrite <- H3.
-                   rewrite of_list_freeVars_vars. reflexivity.
-                 }
-                 rewrite fst_combine, snd_combine; eauto.
-                 rewrite AL; eauto.
-               ++ rewrite fst_combine, snd_combine; eauto.
-                 rewrite disj_minus_eq; eauto.
-                 erewrite <- lookup_list_var_map; eauto.
-                 eapply update_with_list_agree; eauto with len.
-                 symmetry.
-                 eapply agree_on_incl; eauto. eauto with cset.
-                 rewrite H9. clear - H5. cset_tac.
-               ++ clear - H9 H5. cset_tac.
-            -- eapply defined_on_update_list; eauto with len.
-               assert (getAnn al \ of_list Z0 ⊆ lv). {
-                 rewrite <- H1. rewrite <- INCL. clear. cset_tac.
-               }
-               eauto using defined_on_incl.
-        - exploit (@list_to_stmt_correct
-                     ((proj1_sig lreg, lstmp)
-                        :: Parmov.parmove2 positive var_dec (fun _ : positive => pmtmp)
-                        (repl Y' (proj1_sig lreg) lstmp)
-                        (repl Z0 (proj1_sig lreg) lstmp) ++ (lstmp, proj1_sig lreg) :: nil)
-                     (stmtApp l nil) E' L'). {
-            unfold Parmov.parmove2.
-            simpl. rewrite moves_source_set_app; simpl.
-            rewrite !parmove_src_set. simpl. rewrite fst_combine; eauto with len.
-            edestruct (least_fresh_P_full_spec (part_1 p) (blv \ of_list Z0 ∪ lv)); dcr.
-            exploit (H10 (proj1_sig lreg)).
-            - subst lreg. destr_sig. eauto.
-            - subst lreg. destr_sig; dcr. simpl in *; dcr.
-              exploit (H12 (least_fresh_P (part_1 p) (blv \ of_list Z0 ∪ lv))); eauto.
-              + destruct H13; eauto. invc H13. subst reg.
-                set (reg:=least_fresh_P (part_1 p) (blv \ of_list Z0 ∪ lv)) in *.
-                exfalso. eapply NOTCOND.
-                eapply Pos.lt_eq_cases. eapply H12. eauto.
-            - rewrite of_list_repl_incl.
-              eapply defined_on_incl.
-              eapply defined_on_agree_eq; eauto.
-              eapply Ops.freeVars_live_list in H3.
-              rewrite <- of_list_freeVars_vars in H3. rewrite H3.
-              assert (IN:proj1_sig lreg ∈ lv). {
-                rewrite filter_incl in H9. rewrite H1 in H9.
-                clear - H9; cset_tac. eauto.
-              }
-              clear - IN. cset_tac.
-          }
-          pfold. eapply SimSilent.
-          * eapply plus2O. econstructor; eauto with len. reflexivity.
-          * eapply star2_plus2_plus2 with (A:=nil) (B:=nil); eauto.
-            eapply plus2O. econstructor; eauto. reflexivity. reflexivity.
-          * right; eapply pmSim_sim; try eapply LA1; eauto; simpl.
-            -- eapply (inRel_drop LA H4).
-            -- assert (getAnn al ⊆ blv) by eauto with cset.
                symmetry. etransitivity. {
-                 eapply agree_on_incl.
-                 symmetry.
-                 eapply parmov_repl_agree; eauto.
-                 rewrite AL. eauto. rewrite AL; eauto.
-                 instantiate (1:=blv).
-                 rewrite H9. clear - H5 H6. cset_tac.
+                 eapply parmove_elim_mem2mem_agree.
+                 admit.
                }
                eapply agree_on_incl.
                etransitivity.
@@ -666,8 +812,166 @@ Proof.
                  eapply update_with_list_agree; eauto with len.
                  symmetry.
                  eapply agree_on_incl; eauto. eauto with cset.
-                 rewrite H9. clear - H5. cset_tac.
-               ++ clear - H9 H5. cset_tac.
+                 rewrite H10. clear - H5. cset_tac.
+               ++ instantiate (1:=getAnn al).
+                 clear - H10 H5. cset_tac.
+               ++ clear - H7. cset_tac.
+            -- eapply defined_on_update_list; eauto with len.
+               assert (getAnn al \ of_list Z0 ⊆ lv). {
+                 rewrite <- H1. rewrite <- INCL. clear. cset_tac.
+               }
+               eauto using defined_on_incl.
+        - exploit (@list_to_stmt_correct
+                     (parmove_elim_mem2mem
+                        p reg2
+                        (Parmov.parmove2 positive var_dec (fun _ => pmtmp) Y' (repl Z0 reg2 lstmp)) ++
+                        (lstmp, reg2) :: nil)
+                     (stmtApp l nil) E' L'). {
+            unfold Parmov.parmove2.
+            simpl. rewrite moves_source_set_app; simpl.
+            eapply Ops.freeVars_live_list in H3.
+            rewrite <- of_list_freeVars_vars in H3.
+            assert (IN:reg2 ∈ of_list Z0). {
+              edestruct (least_fresh_P_full_spec (part_1 p) (lv)); dcr.
+              edestruct (least_fresh_P_full_spec (part_1 p) (blv ∪ lv)); dcr.
+              subst reg reg2.
+              set (reg:=least_fresh_P (part_1 p) (blv ∪ lv)) in *.
+              set (reg2:=least_fresh_P (part_1 p) lv) in *.
+              exploit (H14 reg2); eauto.
+              simpl.
+              eapply Pos.le_lt_trans; eauto.
+              eapply Pos.lt_nle. eauto. rewrite filter_incl in H13; eauto.
+              clear - H13 H9 AL H1. clearbody reg2. cset_tac'.
+              decide (reg2 ∈ of_list Z0); eauto. cset_tac.
+            }
+            assert (reg2 ∉ of_list Y'). {
+              edestruct (least_fresh_P_full_spec (part_1 p) (lv)); dcr.
+              rewrite H3. eauto.
+            }
+            rewrite !moves_source_set_elim_mem2mem.
+            rewrite !parmove_src_set. simpl. rewrite fst_combine; eauto with len.
+            eapply defined_on_incl.
+            eapply defined_on_agree_eq; eauto.
+            rewrite H3.
+            rewrite <- moves_dest_set_elim_mem2mem.
+            rewrite <- parmove_dest_set;
+              try rewrite fst_combine; try rewrite snd_combine; eauto with len.
+            rewrite of_list_repl_eq; eauto. clear - H3. cset_tac'.
+            rewrite of_list_repl_eq; eauto. clear - NEQ2 H5 AL; cset_tac.
+            - rewrite fst_parmove, snd_parmove, fst_combine, snd_combine; eauto with len.
+              rewrite !of_list_repl.
+              admit.
+          }
+           pfold. eapply SimSilent.
+          * eapply plus2O. econstructor; eauto with len. reflexivity.
+          * eapply star2_plus2_plus2 with (A:=nil) (B:=nil); eauto.
+            eapply plus2O. econstructor; eauto. reflexivity. reflexivity.
+          * right; eapply pmSim_sim; try eapply LA1; eauto; simpl.
+            -- eapply (inRel_drop LA H4).
+            -- assert (getAnn al ⊆ blv) by eauto with cset.
+               symmetry. etransitivity. {
+                 eapply agree_on_incl.
+                 symmetry.
+                 eapply parmov_repl_agree; eauto.
+                 rewrite AL. eauto. rewrite AL; eauto.
+                 instantiate (1:=blv).
+                 rewrite H10. clear - H5 H6. cset_tac.
+               }
+               eapply agree_on_incl.
+               etransitivity.
+               eapply (@parmov_update_with_list (getAnn al));
+                 try rewrite eauto.
+               ++ rewrite snd_combine; eauto.
+               ++ assert (of_list Y' ⊆ lv). {
+                   eapply Ops.freeVars_live_list in H3.
+                   rewrite <- H3.
+                   rewrite of_list_freeVars_vars. reflexivity.
+                 }
+                 rewrite fst_combine, snd_combine; eauto.
+                 rewrite AL; eauto.
+               ++ rewrite fst_combine, snd_combine; eauto.
+                 rewrite disj_minus_eq; eauto.
+                 erewrite <- lookup_list_var_map; eauto.
+                 eapply update_with_list_agree; eauto with len.
+                 symmetry.
+                 eapply agree_on_incl; eauto. eauto with cset.
+                 rewrite H10. clear - H5. cset_tac.
+               ++ clear - H10 H5. cset_tac.
+            -- eapply defined_on_update_list; eauto with len.
+               assert (getAnn al \ of_list Z0 ⊆ lv). {
+                 rewrite <- H1. rewrite <- INCL. clear. cset_tac.
+               }
+               eauto using defined_on_incl.
+
+        - exploit (@list_to_stmt_correct
+                     ((proj1_sig lreg, lstmp)
+                        :: parmove_elim_mem2mem p (proj1_sig lreg)
+                        (Parmov.parmove2 positive var_dec (fun _ : positive => pmtmp)
+                        (repl Y' (proj1_sig lreg) lstmp)
+                        (repl Z0 (proj1_sig lreg) lstmp)) ++ (lstmp, proj1_sig lreg) :: nil)
+                     (stmtApp l nil) E' L'). {
+            unfold Parmov.parmove2.
+            simpl. rewrite moves_source_set_app; simpl.
+            rewrite !moves_source_set_elim_mem2mem.
+            rewrite !parmove_src_set. simpl. rewrite fst_combine; eauto with len.
+            edestruct (least_fresh_P_full_spec (part_1 p) (lv)); dcr.
+            exploit (H11 (proj1_sig lreg)).
+            - subst lreg. destr_sig. eauto.
+            - subst lreg. destr_sig; dcr. simpl in *; dcr.
+              exploit (H13 (least_fresh_P (part_1 p) (lv))); eauto.
+              + destruct H14; eauto. invc H14. subst reg.
+                set (reg:=least_fresh_P (part_1 p) (lv)) in *.
+                exfalso. eapply NOTCOND0.
+                eapply Pos.lt_eq_cases. eapply H13. eauto.
+            - rewrite of_list_repl_incl.
+              eapply defined_on_incl.
+              eapply defined_on_agree_eq; eauto.
+              eapply Ops.freeVars_live_list in H3.
+              rewrite <- of_list_freeVars_vars in H3. rewrite H3.
+              subst reg.
+              assert (IN:proj1_sig lreg ∈ lv). {
+                rewrite filter_incl in H10; eauto.
+              }
+              clear - IN. cset_tac.
+            - rewrite fst_parmove, snd_parmove, fst_combine, snd_combine; eauto with len.
+              rewrite !of_list_repl.
+              clear - NEQ3 NEQ4. cset_tac.
+          }
+          pfold. eapply SimSilent.
+          * eapply plus2O. econstructor; eauto with len. reflexivity.
+          * eapply star2_plus2_plus2 with (A:=nil) (B:=nil); eauto.
+            eapply plus2O. econstructor; eauto. reflexivity. reflexivity.
+          * right; eapply pmSim_sim; try eapply LA1; eauto; simpl.
+            -- eapply (inRel_drop LA H4).
+            -- assert (getAnn al ⊆ blv) by eauto with cset.
+               symmetry. etransitivity. {
+                 eapply agree_on_incl.
+                 symmetry.
+                 eapply parmov_repl_agree; eauto.
+                 rewrite AL. eauto. rewrite AL; eauto.
+                 instantiate (1:=blv).
+                 rewrite H10. clear - H5 H6. cset_tac.
+               }
+               eapply agree_on_incl.
+               etransitivity.
+               eapply (@parmov_update_with_list (getAnn al));
+                 try rewrite eauto.
+               ++ rewrite snd_combine; eauto.
+               ++ assert (of_list Y' ⊆ lv). {
+                   eapply Ops.freeVars_live_list in H3.
+                   rewrite <- H3.
+                   rewrite of_list_freeVars_vars. reflexivity.
+                 }
+                 rewrite fst_combine, snd_combine; eauto.
+                 rewrite AL; eauto.
+               ++ rewrite fst_combine, snd_combine; eauto.
+                 rewrite disj_minus_eq; eauto.
+                 erewrite <- lookup_list_var_map; eauto.
+                 eapply update_with_list_agree; eauto with len.
+                 symmetry.
+                 eapply agree_on_incl; eauto. eauto with cset.
+                 rewrite H10. clear - H5. cset_tac.
+               ++ clear - H10 H5. cset_tac.
             -- eapply defined_on_update_list; eauto with len.
                assert (getAnn al \ of_list Z0 ⊆ lv). {
                  rewrite <- H1. rewrite <- INCL. clear. cset_tac.
